Veritas.Verifier.EAC.fst
@@ -783,6 +783,95 @@ let lemma_non_eac_evicted_addm (#p:pos)
       )
   )
 
+let lemma_non_eac_evicted_addb (#p:pos)   
+  (itsl: non_eac_ts_log p{
+    g_hash_verifiable (partition_idx_seq itsl) /\  
+    EACEvicted? (last_valid_eac_state itsl)  /\
+    AddB? (to_vlog_entry (invalidating_log_entry itsl))
+   })
+  : hash_collision_gen = 
+  (* hash verifiable - evict hash and add hash equal *)                          
+  let gl = partition_idx_seq itsl in                           
+  assert(g_hadd gl = g_hevict gl);
+  
+  let st = last_valid_eac_state itsl in   
+  let ee = invalidating_log_entry itsl in
+  assert(eac_add ee st = EACFail);  
+  match st with
+  | EACEvicted m v_e -> (
+    match ee with
+    | NEvict (AddB (k,v) t j) ->
+      assert(v_e <> v || m <> BAdd);
+
+      let tsle = time_seq_ext itsl in
+      let i = max_eac_prefix tsle in
+      let (e,tid) = index itsl i in
+
+      let itsli = its_prefix itsl i in  
+      (* verifier thread state of tid after itsli *)
+      let vsi = verifier_thread_state itsli tid in
+
+      let itsli' = its_prefix itsl (i + 1) in
+      let vsi' = verifier_thread_state itsli tid in    
+      lemma_verifier_thread_state_extend itsli';  
+      assert(vsi' == t_verify_step vsi e);    
+
+      if m <> BAdd then (
+        (* number of blum evicts is the same as blum adds in the first i entries *)
+        lemma_evict_add_count_same_evictedm itsli k;
+        assert(MS.size (ts_add_set_key itsli k) = MS.size (ts_evict_set_key itsli k));
+      
+        (* the ith element is a blum add *)
+        assert(is_blum_add #p (e,tid));
+        lemma_ts_add_set_key_extend itsli;
+        assert(ts_add_set_key itsli' k == ts_add_set_key itsli k);
+        
+        (* the ith element is not a blum evict *)
+        assert(not (is_blum_evict itsl i));
+        lemma_ts_evict_set_key_extend2 itsli';
+        assert(ts_evict_set_key itsli' k == ts_evict_set_key itsli k);
+  
+        (* this implies that the size of the add set after processing (i+1) elements 
+           * is one larger than the evict set at this point *)
+        assert(MS.size (ts_add_set_key itsli' k) = 1 + (MS.size (ts_evict_set_key itsli' k)));
+
+        (* this implies that in the first (i+1) entries there is an element whose membership in 
+           * add multiset is > its membership in evict multiset *)
+        let be = diff_elem (ts_add_set_key itsli' k) (ts_evict_set_key itsli' k) in
+        lemma_mem_key_add_set_same itsli' be;
+        lemma_mem_key_evict_set_same itsli' be;  
+        assert(MS.mem be (ts_add_set itsli') > MS.mem be (ts_evict_set itsli'));
+
+        (* this implies that in the first (i+1) entries there is an element whose membership in 
+           * add multiset is > its membership in evict multiset *)
+        let be = diff_elem (ts_add_set_key itsli' k) (ts_evict_set_key itsli' k) in
+        lemma_mem_key_add_set_same itsli' be;
+        lemma_mem_key_evict_set_same itsli' be;  
+        assert(MS.mem be (ts_add_set itsli') > MS.mem be (ts_evict_set itsli'));
+
+
+        (* from clock orderedness any evict_set entry for be should happen before i *)
+        lemma_evict_before_add2 itsl i;
+        assert(MS.mem be (ts_evict_set itsl) = MS.mem be (ts_evict_set itsli'));
+        assert(MS.mem be (ts_add_set itsli') > MS.mem be (ts_evict_set itsl));
+
+        lemma_mem_monotonic be itsl (i + 1);
+        assert(MS.mem be (ts_add_set itsl) > MS.mem be (ts_evict_set itsl));  
+
+        MS.lemma_not_equal (ts_add_set itsl) (ts_evict_set itsl) be;
+        assert(~ (g_add_set gl == g_evict_set gl));
+  
+
+        lemma_g_hadd_correct gl;
+        lemma_ghevict_correct gl;
+
+        MultiHashCollision (MSCollision (g_add_seq gl) (g_evict_seq gl))
+      )
+      else (
+        admit()
+      )
+  )
+
 let lemma_non_eac_time_seq_implies_hash_collision 
   (#n:pos) 
   (itsl: non_eac_ts_log n{g_hash_verifiable (partition_idx_seq itsl)}): hash_collision_gen = 
@@ -817,7 +906,7 @@ let lemma_non_eac_time_seq_implies_hash_collision
     match ee with 
       | NEvict (Get _ _) -> lemma_non_eac_evicted_requires_key_in_store itsl
       | NEvict (Put _ _) -> lemma_non_eac_evicted_requires_key_in_store itsl
-      | NEvict (AddB _ _ _) -> admit()
+      | NEvict (AddB _ _ _) -> lemma_non_eac_evicted_addb itsl
       | NEvict (AddM (k,v) _) -> lemma_non_eac_evicted_addm itsl
       | Evict (EvictM _ _) _ -> lemma_non_eac_evicted_requires_key_in_store itsl
       | Evict (EvictB _ _) _ -> lemma_non_eac_evicted_requires_key_in_store itsl
